Remove unnecessary semicolons
Semicolon line terminators aren't required in Standard ML except in a
few cases, and it's bad style to leave them there.

Result of running

    find . -name "*Script.sml" -print0 | xargs -0 gawk -i inplace '{
gsub(/;/,""); print }'

on 'compiler' and 'semantics' (don't want to corrupt git!) and then
manually correcting the couple of syntax errors introduced.

compiler/il2_to_il3/proofs/il3_store_propertiesScript.sml
@@ -1,9 +1,9 @@
-open HolKernel boolLib bossLib lcsymtacs il2_to_il3_compilerTheory pred_setTheory finite_mapTheory listTheory pairTheory integerTheory smallstep_il2Theory relationTheory smallstep_il3Theory arithmeticTheory smallstep_vsm0Theory smallstep_il3_clockedTheory smallstep_il2_clockedTheory;
+open HolKernel boolLib bossLib lcsymtacs il2_to_il3_compilerTheory pred_setTheory finite_mapTheory listTheory pairTheory integerTheory smallstep_il2Theory relationTheory smallstep_il3Theory arithmeticTheory smallstep_vsm0Theory smallstep_il3_clockedTheory smallstep_il2_clockedTheory
 
-val _ = new_theory "il3_store_properties";
+val _ = new_theory "il3_store_properties"
 
 val locs_to_map_total_thm = store_thm("locs_to_map_total_thm", ``!P.?m n.locs_to_map P = (m, n)``,
-Induct_on `P` THEN  rw [locs_to_map_def] THEN rw []);
+Induct_on `P` THEN  rw [locs_to_map_def] THEN rw [])
 
 val map_range_thm = prove(``!P n.((SND (make_loc_map P)) = n) ==> !x.(x ∈ FDOM (FST (make_loc_map P))) ==> ((FST (make_loc_map P)) ' x < n)``,
 rw [EQ_IMP_THM]
@@ -14,7 +14,7 @@ THEN rw [make_loc_map_def, locs_to_map_def, get_locations_def]
 
 THEN `?m n.locs_to_map (get_locations P) = (m, n)` by metis_tac [locs_to_map_total_thm]
 THEN Cases_on `h` THEN fs [get_locations_def] THEN fs [make_loc_map_def, locs_to_map_def, get_locations_def] THEN fs [LET_DEF] THEN Cases_on `i ∈ FDOM m` THEN fs [FST, SND] THEN (TRY decide_tac) THEN rw []
-THEN rw [FAPPLY_FUPDATE_THM] THEN res_tac THEN decide_tac));
+THEN rw [FAPPLY_FUPDATE_THM] THEN res_tac THEN decide_tac))
 
 val map_range_2_thm = prove(``!P x.x < (SND (make_loc_map P)) ==> ?k.k ∈ FDOM (FST (make_loc_map P)) /\ ((FST (make_loc_map P)) ' k = x)``,
 
@@ -26,11 +26,11 @@ THEN fs [LET_DEF] THEN rw [] THEN fs []
 
 THEN Cases_on `k = i` THEN REWRITE_TAC [FAPPLY_FUPDATE_THM]
 
-THEN (Cases_on `x = next_loc` THEN fs [] THEN1 metis_tac  [FAPPLY_FUPDATE_THM] THEN `x < next_loc` by decide_tac THEN res_tac THEN metis_tac [map_range_thm]));
+THEN (Cases_on `x = next_loc` THEN fs [] THEN1 metis_tac  [FAPPLY_FUPDATE_THM] THEN `x < next_loc` by decide_tac THEN res_tac THEN metis_tac [map_range_thm]))
 
-val map_fun_def = Define `map_fun m = \x.m ' x`;
+val map_fun_def = Define `map_fun m = \x.m ' x`
 
-val map_fun_exec = prove(``!m x.map_fun m x = m ' x``, REPEAT STRIP_TAC THEN EVAL_TAC);
+val map_fun_exec = prove(``!m x.map_fun m x = m ' x``, REPEAT STRIP_TAC THEN EVAL_TAC)
 
 
 val make_loc_map_inj = store_thm("make_loc_map_inj", ``!P.INJ (map_fun (FST (make_loc_map P))) (FDOM (FST (make_loc_map P))) UNIV``,
@@ -54,14 +54,14 @@ THEN TRY (`m ' y < m ' y` by metis_tac [map_range_thm, FST, SND, make_loc_map_de
 
 THEN TRY (Cases_on `x = i` THEN fs [] THEN rw [])
 
-THEN TRY (`m ' x < m ' x` by metis_tac [map_range_thm, FST, SND, make_loc_map_def] THEN decide_tac));
+THEN TRY (`m ' x < m ' x` by metis_tac [map_range_thm, FST, SND, make_loc_map_def] THEN decide_tac))
 
-val ms_il2_def = Define `ms_il2 P s = (FDOM s = FDOM (FST (make_loc_map P)))`;
+val ms_il2_def = Define `ms_il2 P s = (FDOM s = FDOM (FST (make_loc_map P)))`
 
 val map_deref_thm = store_thm("map_deref_thm", ``!P st x. (ms_il2 P st) /\ x ∈ FDOM st ⇒ (MAP_KEYS (map_fun (FST (make_loc_map P))) st ' ((map_fun (FST (make_loc_map P))) x) = st ' x)``,
-rw [] THEN metis_tac [MAP_KEYS_def, make_loc_map_inj, INJ_SUBSET, ms_il2_def]);
+rw [] THEN metis_tac [MAP_KEYS_def, make_loc_map_inj, INJ_SUBSET, ms_il2_def])
 
-val int_monotonic_thm = store_thm("int_monotonic_thm",``!x y. (&x < &y) ==> (x < y)``, rw []);
+val int_monotonic_thm = store_thm("int_monotonic_thm",``!x y. (&x < &y) ==> (x < y)``, rw [])
 
 val every_store_inc_in_map = prove(``!i P n.((n < LENGTH P) /\ ((P !! &n = IL2_Store i) \/ (P !! &n = IL2_Load i))) ==> i ∈ FDOM (FST (make_loc_map P))``,
 Induct_on `P`
@@ -82,10 +82,10 @@ THEN (TRY (metis_tac []))
 
 THEN rw [locs_to_map_def]
 
-THEN (TRY (Cases_on `i' ∈ FDOM map`)) THEN (TRY (Cases_on `i ∈ FDOM map`)) THEN fs [FST, SND] THEN rw [] THEN (TRY (metis_tac [])) THEN rw [get_locations_def, locs_to_map_def, FST, FAPPLY_FUPDATE_THM] THEN Cases_on `i ∈ FDOM map'` THEN rw [])));
+THEN (TRY (Cases_on `i' ∈ FDOM map`)) THEN (TRY (Cases_on `i ∈ FDOM map`)) THEN fs [FST, SND] THEN rw [] THEN (TRY (metis_tac [])) THEN rw [get_locations_def, locs_to_map_def, FST, FAPPLY_FUPDATE_THM] THEN Cases_on `i ∈ FDOM map'` THEN rw [])))
 
 val ms_il2_trans = store_thm("ms_il2_trans", ``!P r''' i v.ms_il2 P r''' /\ ms_il2 P (r''' |+ (i, v)) ==> (FDOM r''' = FDOM (r''' |+ (i, v)))``,
-metis_tac [ms_il2_def]);
+metis_tac [ms_il2_def])
 
 val ms_const = store_thm("ms_const", ``!P c c'.exec_clocked P c c' ==> !x y.(c = SOME x) /\ (c' = SOME y) ==> ms_il2 P (SND (SND (SND x))) ==> ms_il2 P (SND (SND (SND y)))``,
 fs [exec_clocked_def] THEN STRIP_TAC THEN ho_match_mp_tac RTC_STRONG_INDUCT
@@ -104,9 +104,9 @@ THEN fs [FDOM_FUPDATE]
 
 THEN `i INSERT FDOM (FST (make_loc_map P)) = FDOM (FST (make_loc_map P))` by (rw [INSERT_DEF, EXTENSION] THEN Cases_on `x = i` THEN rw [])
 
-THEN rw []);
+THEN rw [])
 
-val ms_const_2 = store_thm("ms_const_2", ``!P pc c stk st pc' c' stk' st'.exec_clocked_one P (SOME (pc, c, stk, st)) (SOME (pc', c', stk', st')) ==> ms_il2 P st ==> ms_il2 P st'``, metis_tac [ms_const, SND, exec_clocked_def, RTC_SUBSET]);
+val ms_const_2 = store_thm("ms_const_2", ``!P pc c stk st pc' c' stk' st'.exec_clocked_one P (SOME (pc, c, stk, st)) (SOME (pc', c', stk', st')) ==> ms_il2 P st ==> ms_il2 P st'``, metis_tac [ms_const, SND, exec_clocked_def, RTC_SUBSET])
 
 
 val every_store_inc_in_map = prove(``!i P n.((n < LENGTH P) /\ ((P !! &n = IL2_Store i) \/ (P !! &n = IL2_Load i))) ==> i ∈ FDOM (FST (make_loc_map P))``,
@@ -128,22 +128,22 @@ THEN (TRY (metis_tac []))
 
 THEN rw [locs_to_map_def]
 
-THEN (TRY (Cases_on `i' ∈ FDOM map`)) THEN (TRY (Cases_on `i ∈ FDOM map`)) THEN fs [FST, SND] THEN rw [] THEN (TRY (metis_tac [])) THEN rw [get_locations_def, locs_to_map_def, FST, FAPPLY_FUPDATE_THM] THEN Cases_on `i ∈ FDOM map'` THEN rw [])));
+THEN (TRY (Cases_on `i' ∈ FDOM map`)) THEN (TRY (Cases_on `i ∈ FDOM map`)) THEN fs [FST, SND] THEN rw [] THEN (TRY (metis_tac [])) THEN rw [get_locations_def, locs_to_map_def, FST, FAPPLY_FUPDATE_THM] THEN Cases_on `i ∈ FDOM map'` THEN rw [])))
 
-val s_uloc_def = Define `(s_uloc [] = 0) /\ (s_uloc (VSM_Load l::xs) = MAX (l + 1) (s_uloc xs)) /\ (s_uloc (VSM_Store l::xs) = MAX (l+1) (s_uloc xs)) /\ (s_uloc (_::xs) = s_uloc xs)`;
+val s_uloc_def = Define `(s_uloc [] = 0) /\ (s_uloc (VSM_Load l::xs) = MAX (l + 1) (s_uloc xs)) /\ (s_uloc (VSM_Store l::xs) = MAX (l+1) (s_uloc xs)) /\ (s_uloc (_::xs) = s_uloc xs)`
 
 val FETCH_EL = store_thm("FETCH_EL", ``!xs n.n < LENGTH xs ==> (xs !! &n = EL n xs)``,
 Induct_on `n`
 
 THEN1 (rw [fetch_def] THEN Cases_on `xs` THEN fs [LENGTH, fetch_def])
 THEN rw [fetch_def]
-THEN rw [EL] THEN Cases_on `xs` THEN fs [LENGTH] THEN res_tac THEN rw [fetch_def] THEN `&SUC n - 1 = &n` by (fs [INT, int_sub] THEN rw [Once (GSYM INT_ADD_ASSOC)]) THEN rw []);
+THEN rw [EL] THEN Cases_on `xs` THEN fs [LENGTH] THEN res_tac THEN rw [fetch_def] THEN `&SUC n - 1 = &n` by (fs [INT, int_sub] THEN rw [Once (GSYM INT_ADD_ASSOC)]) THEN rw [])
 
 val suloc_thm = store_thm("suloc_thm", ``!P q n.(q < LENGTH P) /\ (P !! &q = VSM_Store n) ==> (n < s_uloc P)``,
 Induct_on `q` THEN rw [] THEN rfs [FETCH_EL] THEN (Cases_on `P` THEN1 (fs [LENGTH]))
 THEN1 (fs [] THEN rw [s_uloc_def])
 THEN
-Cases_on `h` THEN fs [EL, s_uloc_def] THEN rw [] THEN fs [] THEN rw [] THEN res_tac THEN fs [FETCH_EL]);
+Cases_on `h` THEN fs [EL, s_uloc_def] THEN rw [] THEN fs [] THEN rw [] THEN res_tac THEN fs [FETCH_EL])
 
 val suloc_2_thm = prove(``!P a b.exec_il3_c P a b ==> !c c'.(a = SOME c) /\ (b = SOME c') ==> (!l.l ∈ FDOM (SND (SND (SND c))) <=> l < s_uloc P) ==> (!l.l ∈ FDOM (SND (SND (SND c'))) <=> l < s_uloc P)``,
 STRIP_TAC THEN fs [exec_il3_c_def] THEN ho_match_mp_tac RTC_STRONG_INDUCT THEN rw []
@@ -159,33 +159,33 @@ THEN imp_res_tac suloc_thm
 THEN fs [int_monotonic_thm] THEN rfs []
 THEN `!l. (l = n) ==> (l < s_uloc P)` by metis_tac []
 THEN `!l. l ∈ FDOM r' ⇔ l < s_uloc P` by metis_tac [EQ_IMP_THM]
-THEN metis_tac []);
+THEN metis_tac [])
 
 val suloc_21_thm = store_thm("suloc_21_thm", ``!P pc c stk st pc' c' stk' st'.exec_il3_c P (SOME (pc, c, stk, st)) (SOME (pc', c', stk', st')) /\ (!l.l ∈ FDOM st <=> l < s_uloc P) ==> (!l.l ∈ FDOM st' <=> l < s_uloc P)``,
 rw []
 THEN mp_tac suloc_2_thm
 THEN rw []
 THEN res_tac
-THEN fs [SND]);
+THEN fs [SND])
 
 val stack_contains_store_def = Define `
 stack_contains_store st stk = !l.l ∈ FDOM st ==> (l < LENGTH stk) /\ (stk ?? l = st ' l)
-`;
+`
 
 val drop_thm = store_thm("drop_thm", ``!xs ys.DROP (LENGTH xs) (xs ++ ys) = ys``,
-Induct_on `xs` THEN rw []);
+Induct_on `xs` THEN rw [])
 
 val take_thm = store_thm("take_thm", ``!xs ys.TAKE (LENGTH xs) (xs ++ ys) = xs``,
-Induct_on `xs` THEN rw []);
+Induct_on `xs` THEN rw [])
 
 
-val astack_def = Define `astack P st stk = stk ++ (REVERSE (GENLIST (\l.st ' l) (s_uloc P)))`;
+val astack_def = Define `astack P st stk = stk ++ (REVERSE (GENLIST (\l.st ' l) (s_uloc P)))`
 
 val astack_produces_valid_store = store_thm("astack_produces_valid_store", ``!P st stk.(!l.l ∈ FDOM st <=> l < s_uloc P) ==> ?n.(stk = TAKE n (astack P st stk)) /\ stack_contains_store st (DROP n (astack P st stk))``,
 
 rw [astack_def]
 THEN EXISTS_TAC ``(LENGTH stk)`` THEN
-rw [take_thm, drop_thm, stack_contains_store_def, fetch_rev_def, FETCH_EL, LESS_EQ_IMP_LESS_SUC]);
+rw [take_thm, drop_thm, stack_contains_store_def, fetch_rev_def, FETCH_EL, LESS_EQ_IMP_LESS_SUC])
 
 
 val load_in_prog_imp_in_map = prove(``!P i'.MEM (IL2_Load i') P ==> i' ∈ FDOM (FST (make_loc_map P)) ``,
@@ -193,20 +193,20 @@ Induct_on `P` THEN rw [] THEN fs [MEM, FST, make_loc_map_def, locs_to_map_def, g
 THEN (TRY (res_tac THEN Cases_on `h` THEN fs [fetch_def, make_loc_map_def, il2_to_il3_def, s_uloc_def, locs_to_map_def, get_locations_def, il2_to_il3m_def, FCARD_FEMPTY]))
 
 THEN `?m n.locs_to_map (get_locations P) = (m, n)` by metis_tac [locs_to_map_total_thm] THEN fs [LET_DEF]
-THEN Cases_on `i' ∈ FDOM m` THEN fs [] THEN rw []);
+THEN Cases_on `i' ∈ FDOM m` THEN fs [] THEN rw [])
 
 val store_in_prog_imp_in_map = prove(``!P i'.MEM (IL2_Store i') P ==> i' ∈ FDOM (FST (make_loc_map P)) ``,
 Induct_on `P` THEN rw [] THEN fs [MEM, FST, make_loc_map_def, locs_to_map_def, get_locations_def]
 THEN (TRY (res_tac THEN Cases_on `h` THEN fs [fetch_def, make_loc_map_def, il2_to_il3_def, s_uloc_def, locs_to_map_def, get_locations_def, il2_to_il3m_def, FCARD_FEMPTY]))
 
 THEN `?m n.locs_to_map (get_locations P) = (m, n)` by metis_tac [locs_to_map_total_thm] THEN fs [LET_DEF]
-THEN Cases_on `i' ∈ FDOM m` THEN fs [] THEN rw []);
+THEN Cases_on `i' ∈ FDOM m` THEN fs [] THEN rw [])
 
 
 val snd_arg_fcard = prove(``!P.SND (make_loc_map P) = FCARD (FST (make_loc_map P))``,
 
 fs [make_loc_map_def] THEN Induct_on `P` THEN rw [get_locations_def, locs_to_map_def, FST, FCARD_FEMPTY] THEN Cases_on `h` THEN  fs [fetch_def, make_loc_map_def, il2_to_il3_def, s_uloc_def, locs_to_map_def, get_locations_def, il2_to_il3m_def] THEN `?m n.locs_to_map (get_locations P) = (m, n)` by metis_tac [locs_to_map_total_thm] THEN fs [LET_DEF]
-THEN Cases_on `i ∈ FDOM m` THEN fs [FCARD_FUPDATE] THEN decide_tac);
+THEN Cases_on `i ∈ FDOM m` THEN fs [FCARD_FUPDATE] THEN decide_tac)
 
 val s_uloc_fcard = prove(``!P.s_uloc (il2_to_il3 P) = FCARD (FST (make_loc_map P))``,
 
@@ -243,9 +243,9 @@ THEN rw []
 
 THEN rw [MAX_DEF]
 
-THEN `FCARD m = n` by metis_tac [snd_arg_fcard, FST, make_loc_map_def, SND, MAX_DEF] THEN decide_tac);
+THEN `FCARD m = n` by metis_tac [snd_arg_fcard, FST, make_loc_map_def, SND, MAX_DEF] THEN decide_tac)
 
-val least_unused_loc_is_next_to_use = prove(``!P.SND (make_loc_map P) = s_uloc (il2_to_il3 P)``, metis_tac [s_uloc_fcard, snd_arg_fcard]);
+val least_unused_loc_is_next_to_use = prove(``!P.SND (make_loc_map P) = s_uloc (il2_to_il3 P)``, metis_tac [s_uloc_fcard, snd_arg_fcard])
 
 val min_store_imp_all_locs_in_range = store_thm("min_store_imp_all_locs_in_range", ``!P st.ms_il2 P st ==> (!l.l ∈ FDOM (MAP_KEYS (map_fun (FST (make_loc_map P))) st) <=> (l < s_uloc (il2_to_il3 P)))``,
 
@@ -255,6 +255,6 @@ THEN rw [MAP_KEYS_def, make_loc_map_inj]
 
 THEN `s_uloc (il2_to_il3 P) = (SND (make_loc_map P))` by metis_tac [least_unused_loc_is_next_to_use]
 
-THEN metis_tac [locs_to_map_total_thm, map_fun_def, map_range_thm, make_loc_map_def,EQ_IMP_THM, map_range_2_thm, FST, SND, make_loc_map_def]);
+THEN metis_tac [locs_to_map_total_thm, map_fun_def, map_range_thm, make_loc_map_def,EQ_IMP_THM, map_range_2_thm, FST, SND, make_loc_map_def])
 
-val _ = export_theory ();
+val _ = export_theory ()
