compiler/l1_to_il1/proof/comp_locationScript.sml
@@ -1,6 +1,6 @@
-open HolKernel boolLib bossLib listTheory Parse IndDefLib finite_mapTheory relationTheory arithmeticTheory ast_il1Theory bigstep_il1Theory pred_setTheory pairTheory lcsymtacs prim_recTheory integerTheory store_equivalenceTheory l1_to_il1_compilerTheory l1_il1_totalTheory;
+open HolKernel boolLib bossLib listTheory Parse IndDefLib finite_mapTheory relationTheory arithmeticTheory ast_il1Theory bigstep_il1Theory pred_setTheory pairTheory lcsymtacs prim_recTheory integerTheory store_equivalenceTheory l1_to_il1_compilerTheory l1_il1_totalTheory
 
-val _ = new_theory "comp_location";
+val _ = new_theory "comp_location"
 
 val count_assign_def = Define `
 (count_assign (IL1_Expr _) _ = Num 0) /\
@@ -8,14 +8,14 @@ val count_assign_def = Define `
 (count_assign (IL1_While _ e2) l = count_assign e2 l) /\
 (count_assign (IL1_Assign l1 e) l2 = if l1 = l2 then Num 1 else Num 0) /\
 (count_assign (IL1_Seq e1 e2) l = count_assign e1 l + count_assign e2 l) /\
-(count_assign (IL1_Tick e) l = count_assign e l)`;
+(count_assign (IL1_Tick e) l = count_assign e l)`
 
 val count_deref_expr_def = Define `
 (count_deref_expr (IL1_Deref l) l' = if l = l' then Num 1 else Num 0) /\
 (count_deref_expr (IL1_Value _) _ = Num 0) /\
 (count_deref_expr (IL1_Plus e1 e2) l = count_deref_expr e1 l + count_deref_expr e2 l) /\
 (count_deref_expr (IL1_Geq e1 e2) l = count_deref_expr e1 l + count_deref_expr e2 l) /\
-(count_deref_expr (IL1_EIf e1 e2 e3) l = count_deref_expr e1 l + count_deref_expr e2 l + count_deref_expr e3 l)`;
+(count_deref_expr (IL1_EIf e1 e2 e3) l = count_deref_expr e1 l + count_deref_expr e2 l + count_deref_expr e3 l)`
 
 val count_deref_def = Define `
 (count_deref (IL1_Expr e) l = count_deref_expr e l) /\
@@ -23,10 +23,10 @@ val count_deref_def = Define `
 (count_deref (IL1_While e1 e2) l = count_deref_expr e1 l + count_deref e2 l) /\
 (count_deref (IL1_Assign l1 e) l2 = count_deref_expr e l2) /\
 (count_deref (IL1_Seq e1 e2) l = count_deref e1 l + count_deref e2 l) /\
-(count_deref (IL1_Tick e) l = count_deref e l)`;
+(count_deref (IL1_Tick e) l = count_deref e l)`
 
 val CONTAINS_SIMPED_THM = store_thm("CONTAINS_SIMPED_THM",
-``!n e st ex n' l.(l1_to_il1_pair n e = (st, ex, n')) ==> (contains_a l (l1_to_il1 e n) <=> contains_a l st)``, rfs [EQ_IMP_THM,l1_to_il1_def, LET_DEF, contains_a_def]);
+``!n e st ex n' l.(l1_to_il1_pair n e = (st, ex, n')) ==> (contains_a l (l1_to_il1 e n) <=> contains_a l st)``, rfs [EQ_IMP_THM,l1_to_il1_def, LET_DEF, contains_a_def])
 
 val COMP_LOC_INCREASING_THM = store_thm("COMP_LOC_INCREASING_THM",
 ``!e n n' sl1 e1'.(l1_to_il1_pair n e = (sl1, e1', n')) ==> (n' >= n)``,
@@ -39,7 +39,7 @@ fs [LET_DEF, l1_to_il1_pair_def] THEN
 res_tac THEN
 decide_tac)
 THEN1 ((`?sl1 e1' n''.l1_to_il1_pair n' e = (sl1, e1', n'')` by metis_tac [L1_TO_IL1_TOTAL_THM]) THEN fs [l1_to_il1_pair_def, LET_DEF])
-);
+)
 
 val COMPILER_LOC_CHANGE_THM = store_thm("COMPILER_LOC_CHANGE_THM",
 ``!st ex n n' e.(l1_to_il1_pair n e = (st, ex, n')) ==> (n <> n') ==> contains_a (Compiler n) (l1_to_il1 e n)``,
@@ -65,7 +65,7 @@ THEN FAIL_TAC "expect to fail")
 THEN1 (`?st ex rl.l1_to_il1_pair n' e = (st, ex, rl)` by metis_tac [L1_TO_IL1_TOTAL_THM]
 THEN fs [LET_DEF, l1_to_il1_def, l1_to_il1_pair_def]
 THEN rw []
-THEN fs [contains_a_def]));
+THEN fs [contains_a_def]))
 
 val ALL_CO_LOCS_IN_RANGE_BA = store_thm("ALL_CO_LOCS_IN_RANGE_BA",
 ``!e n st ex n' tn.(l1_to_il1_pair n e = (st, ex, n')) ==> contains (Compiler tn) (l1_to_il1 e n) ==> (tn >= n) /\ (tn < n')``,
@@ -82,7 +82,7 @@ THEN `?st' ex' rl'.l1_to_il1_pair rl e' = (st', ex', rl')` by metis_tac [L1_TO_I
 THEN `?st'' ex'' rl''.l1_to_il1_pair rl' e'' = (st'', ex'', rl'')` by metis_tac [L1_TO_IL1_TOTAL_THM]
 THEN `?st'' ex'' rl''.l1_to_il1_pair rl' e = (st'', ex'', rl'')` by metis_tac [L1_TO_IL1_TOTAL_THM]
 THEN fs [l1_to_il1_def, l1_to_il1_pair_def, LET_DEF, contains_def, contains_expr_def] THEN rw [] THEN imp_res_tac COMP_LOC_INCREASING_THM THEN res_tac THEN decide_tac)
-THEN `?st ex rl.l1_to_il1_pair n' e = (st, ex, rl)` by metis_tac [L1_TO_IL1_TOTAL_THM] THEN fs [l1_to_il1_def, l1_to_il1_pair_def, LET_DEF, contains_def, contains_expr_def] THEN rw [] THEN imp_res_tac COMP_LOC_INCREASING_THM THEN res_tac THEN decide_tac);
+THEN `?st ex rl.l1_to_il1_pair n' e = (st, ex, rl)` by metis_tac [L1_TO_IL1_TOTAL_THM] THEN fs [l1_to_il1_def, l1_to_il1_pair_def, LET_DEF, contains_def, contains_expr_def] THEN rw [] THEN imp_res_tac COMP_LOC_INCREASING_THM THEN res_tac THEN decide_tac)
 
 val ALL_CO_LOCS_IN_RANGE_FOR = store_thm("ALL_CO_LOCS_IN_RANGE_FOR",
 ``!e n st ex n'.(l1_to_il1_pair n e = (st, ex, n')) ==> !n''.(n'' >= n) /\ (n'' < n') ==> contains_a (Compiler n'') (l1_to_il1 e n)``,
@@ -132,19 +132,19 @@ Cases_on `n'' < rl` THEN fs [contains_a_def] THEN rw []
 THEN fs [NOT_LESS]
 THEN Cases_on `n'' = rl''` THEN rw []
 THEN `n'' < n'` by decide_tac
-THEN metis_tac [COMP_LOC_INCREASING_THM, GREATER_EQ, NOT_LESS_EQUAL]));
+THEN metis_tac [COMP_LOC_INCREASING_THM, GREATER_EQ, NOT_LESS_EQUAL]))
 
 val CONTAINS_IMPLIES_COUNT_NZERO = store_thm("CONTAINS_IMPLIES_COUNT_NZERO",
 ``!e l.contains_a l e <=> (count_assign e l <> 0)``,
-rw [EQ_IMP_THM] THEN Induct_on `e` THEN rw [contains_a_def, count_assign_def] THEN metis_tac []);
+rw [EQ_IMP_THM] THEN Induct_on `e` THEN rw [contains_a_def, count_assign_def] THEN metis_tac [])
 
 val ALL_CO_LOCS_IN_RANGE = store_thm("ALL_CO_LOCS_IN_RANGE",
 ``!e n st ex n' tn.(l1_to_il1_pair n e = (st, ex, n')) ==> (contains (Compiler tn) (l1_to_il1 e n) <=> (tn >= n) /\ (tn < n'))``,
-metis_tac [EQ_IMP_THM, ALL_CO_LOCS_IN_RANGE_BA, ALL_CO_LOCS_IN_RANGE_FOR, CONTAINS_A_SUB]);
+metis_tac [EQ_IMP_THM, ALL_CO_LOCS_IN_RANGE_BA, ALL_CO_LOCS_IN_RANGE_FOR, CONTAINS_A_SUB])
 
 val UNCHANGED_LOC_SIMP_THM = store_thm("UNCHANGED_LOC_SIMP_THM",
 ``!n e st ex n' tn.(l1_to_il1_pair n e = (st,ex,n')) ⇒
      (contains_a (Compiler tn) st ⇔ tn ≥ n ∧ tn < n')``,
-rw [EQ_IMP_THM] THEN metis_tac [CONTAINS_SIMPED_THM, ALL_CO_LOCS_IN_RANGE_BA, CONTAINS_A_SUB, ALL_CO_LOCS_IN_RANGE_FOR]);
+rw [EQ_IMP_THM] THEN metis_tac [CONTAINS_SIMPED_THM, ALL_CO_LOCS_IN_RANGE_BA, CONTAINS_A_SUB, ALL_CO_LOCS_IN_RANGE_FOR])
 
-val _ = export_theory ();
+val _ = export_theory ()
