compiler/l1_to_il1/proof/store_equivalenceScript.sml
@@ -1,13 +1,13 @@
-open HolKernel boolLib bossLib listTheory Parse IndDefLib finite_mapTheory relationTheory arithmeticTheory ast_il1Theory bigstep_il1_clockedTheory pred_setTheory pairTheory lcsymtacs prim_recTheory integerTheory;
+open HolKernel boolLib bossLib listTheory Parse IndDefLib finite_mapTheory relationTheory arithmeticTheory ast_il1Theory bigstep_il1_clockedTheory pred_setTheory pairTheory lcsymtacs prim_recTheory integerTheory
 
-val _ = new_theory "store_equivalence";
+val _ = new_theory "store_equivalence"
 
 val contains_expr_def = Define `
     (contains_expr l (IL1_Value v) = F) /\
     (contains_expr l (IL1_Plus e1 e2) = contains_expr l e1 \/ contains_expr l e2) /\
     (contains_expr l (IL1_Geq e1 e2) = contains_expr l e1 \/ contains_expr l e2) /\
     (contains_expr l1 (IL1_Deref l2) = (l1 = l2)) /\
-    (contains_expr l (IL1_EIf e1 e2 e3) = contains_expr l e1 \/ contains_expr l e2 \/ contains_expr l e3)`;
+    (contains_expr l (IL1_EIf e1 e2 e3) = contains_expr l e1 \/ contains_expr l e2 \/ contains_expr l e3)`
 
 val contains_def = Define `
     (contains l (IL1_Expr e) = contains_expr l e) /\
@@ -15,7 +15,7 @@ val contains_def = Define `
     (contains l (IL1_Seq e1 e2) = contains l e1 \/ contains l e2) /\
     (contains l (IL1_SIf e1 e2 e3) = contains_expr l e1 \/ contains l e2 \/ contains l e3) /\
     (contains l (IL1_While e1 e2) = contains_expr l e1 \/ contains l e2) /\
-    (contains l (IL1_Tick e) = contains l e)`;
+    (contains l (IL1_Tick e) = contains l e)`
 
 val contains_a_def = Define `
     (contains_a l (IL1_Expr _) = F) /\
@@ -23,25 +23,25 @@ val contains_a_def = Define `
     (contains_a l (IL1_Seq e1 e2) = contains_a l e1 \/ contains_a l e2) /\
     (contains_a l (IL1_SIf _ e2 e3) = contains_a l e2 \/ contains_a l e3) /\
     (contains_a l (IL1_While _ e2) = contains_a l e2) /\
-    (contains_a l (IL1_Tick e) = contains_a l e)`;
+    (contains_a l (IL1_Tick e) = contains_a l e)`
 
 val CONTAINS_A_SUB = store_thm("CONTAINS_A_SUB",
 ``!l e.contains_a l e ==> contains l e``,
-Induct_on `e` THEN metis_tac [contains_a_def, contains_def]);
+Induct_on `e` THEN metis_tac [contains_a_def, contains_def])
 
-val equiv_def = Define `equiv s1 s2 = (!k.User k ∈ FDOM s1 <=> User k ∈ FDOM s2) /\ (!k.(User k ∈ FDOM s1 \/ User k ∈ FDOM s2) ==> (s1 ' (User k) = s2 ' (User k)))`;
+val equiv_def = Define `equiv s1 s2 = (!k.User k ∈ FDOM s1 <=> User k ∈ FDOM s2) /\ (!k.(User k ∈ FDOM s1 \/ User k ∈ FDOM s2) ==> (s1 ' (User k) = s2 ' (User k)))`
 
 val EQUIV_REFL_THM = store_thm("EQUIV_REFL_THM",
 ``!x.equiv x x``,
-fs [equiv_def]);
+fs [equiv_def])
 
 val EQUIV_TRANS_THM = store_thm("EQUIV_TRANS_THM",
 ``!x y z.equiv x y /\ equiv y z ==> equiv x z``,
-rw [equiv_def]);
+rw [equiv_def])
 
 val EQUIV_APPEND_THM = store_thm("EQUIV_APPEND_THM",
 ``!e1 e2 k v.equiv e1 e2 ==> equiv (e1 |+ (k, v)) (e2 |+ (k, v))``,
-rw [equiv_def] THEN metis_tac [FST, FUPDATE_SAME_APPLY]);
+rw [equiv_def] THEN metis_tac [FST, FUPDATE_SAME_APPLY])
 
 val MAP_APPEND_EQUIV_THM = store_thm("MAP_APPEND_EQUIV_THM",
 ``!s k v.(MAP_KEYS User s) |+ (User k, v) = (MAP_KEYS User (s |+ (k, v)))``,
@@ -50,22 +50,22 @@ THEN metis_tac [MAP_KEYS_FUPDATE])
 
 val EQUIV_SYM_THM = store_thm("EQUIV_SYM_THM",
 ``!s s'.equiv s s' <=> equiv s' s``,
-metis_tac [equiv_def]);
+metis_tac [equiv_def])
 
 val STORE_L1_IL1_INJ = store_thm("STORE_L1_IL1_INJ",
 ``!l s. l ∈ FDOM s ==> ((s ' l) = (MAP_KEYS User s) ' (User l))``,
 rw [] THEN `FDOM (MAP_KEYS User s) = IMAGE User (FDOM s)` by rw [FDOM_DEF, MAP_KEYS_def, IMAGE_DEF]
-THEN `INJ User (FDOM s) UNIV` by rw [INJ_DEF] THEN metis_tac [MAP_KEYS_def]);
+THEN `INJ User (FDOM s) UNIV` by rw [INJ_DEF] THEN metis_tac [MAP_KEYS_def])
 
-val con_store_def = Define `con_store s = MAP_KEYS User s`;
+val con_store_def = Define `con_store s = MAP_KEYS User s`
 
 val NOT_CONTAINS_MEANS_UNCHANGED_LEMMA = prove(
 ``!c p r.bs_il1_c c p r ==> !x.(r = SOME x) ==> !l.~contains_a l (FST p) ==> (((SND p) ' l) = ((FST (SND x)) ' l))``,
-ho_match_mp_tac bs_il1_c_strongind THEN rw [] THEN fs [FST, SND] THEN fs [contains_a_def] THEN metis_tac [FAPPLY_FUPDATE_THM]);
+ho_match_mp_tac bs_il1_c_strongind THEN rw [] THEN fs [FST, SND] THEN fs [contains_a_def] THEN metis_tac [FAPPLY_FUPDATE_THM])
 
 val NOT_CONTAINS_MEANS_UNCHANGED_THM = store_thm("NOT_CONTAINS_MEANS_UNCHANGED_THM",
 ``!c c' e s v s'.bs_il1_c c (e, s) (SOME (v, s', c')) ==> !l.~contains_a l e ==> (s ' l = s' ' l)``,
-metis_tac [NOT_CONTAINS_MEANS_UNCHANGED_LEMMA, FST, SND]);
+metis_tac [NOT_CONTAINS_MEANS_UNCHANGED_LEMMA, FST, SND])
 
 
-val _ = export_theory ();
+val _ = export_theory ()
