compiler/l1_to_il1/proof/l1_il1_totalScript.sml
@@ -1,6 +1,6 @@
-open HolKernel boolLib bossLib listTheory Parse IndDefLib finite_mapTheory relationTheory arithmeticTheory ast_il1Theory bigstep_il1Theory pred_setTheory pairTheory lcsymtacs prim_recTheory integerTheory store_equivalenceTheory l1_to_il1_compilerTheory;
+open HolKernel boolLib bossLib listTheory Parse IndDefLib finite_mapTheory relationTheory arithmeticTheory ast_il1Theory bigstep_il1Theory pred_setTheory pairTheory lcsymtacs prim_recTheory integerTheory store_equivalenceTheory l1_to_il1_compilerTheory
 
-val _ = new_theory "l1_il1_total";
+val _ = new_theory "l1_il1_total"
 
 val L1_TO_IL1_TOTAL_THM = store_thm("L1_TO_IL1_TOTAL_THM",
 ``!e n.?sl e' lc.l1_to_il1_pair n e = (sl, e', lc)``,
@@ -14,6 +14,6 @@ THEN
 `?sl e' lc.l1_to_il1_pair n e = (sl, e', lc)` by METIS_TAC [] THEN
 `?sl e'' lc'.l1_to_il1_pair lc e' = (sl, e'', lc')` by METIS_TAC [] THEN
 `?sl e''' lc''.l1_to_il1_pair lc' e = (sl, e''', lc'')` by METIS_TAC []
-THEN rw []);
+THEN rw [])
 
-val _ = export_theory ();
+val _ = export_theory ()
