semantics/l1/proofs/smallstep_progressScript.sml
@@ -1,10 +1,10 @@
-open HolKernel Parse boolLib bossLib integerTheory finite_mapTheory ast_l1Theory smallstep_l1Theory lcsymtacs pairTheory l1_typeTheory pred_setTheory;
+open HolKernel Parse boolLib bossLib integerTheory finite_mapTheory ast_l1Theory smallstep_l1Theory lcsymtacs pairTheory l1_typeTheory pred_setTheory
 
-val _ = new_theory "smallstep_progress";
+val _ = new_theory "smallstep_progress"
 
 val L1_PROGRESS_THM = store_thm("L1_PROGRESS_THM",
 ``!e g t.l1_type e g t ==> !s.g ⊆ (FDOM s) ==> (?v.e = L1_Value v) \/ (?e' s'.ss_l1 (e, s) (e', s'))``,
 ho_match_mp_tac l1_type_strongind
-THEN rw [] THEN rw [Once ss_l1_cases] THEN fs [Once l1_type_cases] THEN rw [] THEN metis_tac [SUBSET_DEF]);
+THEN rw [] THEN rw [Once ss_l1_cases] THEN fs [Once l1_type_cases] THEN rw [] THEN metis_tac [SUBSET_DEF])
 
-val _ = export_theory ();
+val _ = export_theory ()
