semantics/vsm0/ast_vsm0Script.sml
@@ -1,8 +1,8 @@
-open HolKernel bossLib Parse integerTheory;
+open HolKernel bossLib Parse integerTheory
 
-val _ = new_theory "ast_vsm0";
+val _ = new_theory "ast_vsm0"
 
-val _ = type_abbrev("vsm_loc", ``:num``);
+val _ = type_abbrev("vsm_loc", ``:num``)
 
 val _ = Datatype `vsm_stm = VSM_Nop
                           | VSM_Tick
@@ -14,8 +14,8 @@ val _ = Datatype `vsm_stm = VSM_Nop
                           | VSM_Geq
                           | VSM_Halt
                           | VSM_Jump int
-                          | VSM_Jz int`;
+                          | VSM_Jz int`
 
-val _ = type_abbrev("vsm_prog", ``:(vsm_stm list)``);
+val _ = type_abbrev("vsm_prog", ``:(vsm_stm list)``)
 
-val _ = export_theory ();
+val _ = export_theory ()
